{
 "cells": [
  {
   "cell_type": "markdown",
   "metadata": {},
   "source": [
    "# Exercise 03.a: Stability of the advection equation\n",
    "\n",
    "**Due:** _15 December 2020_"
   ]
  },
  {
   "cell_type": "markdown",
   "metadata": {},
   "source": [
    "**Names:** Linus, Lukas, David, Mariana "
   ]
  },
  {
   "cell_type": "markdown",
   "metadata": {},
   "source": [
    "Analyze the stability of the following finite difference approximations to the one dimensional advection equation\n",
    "$$u_t + cu_x=0$$\n",
    "\n",
    "1. Leap frog in time, centred in space\n",
    "1. Forward in time, upstream\n",
    "1. Forward in time, downstream\n",
    "\n",
    "Hint: write $u^n_j = A\\lambda^n{\\rm e}^{ikj\\Delta x}$ in the finite difference approximation\n",
    "and solve the resulting equation for $\\lambda$. The difference scheme is stable\n",
    "if $\\vert\\lambda\\vert \\le 1$. Note that $A$ is a constant.\n"
   ]
  },
  {
   "cell_type": "markdown",
   "metadata": {},
   "source": [
    "## 3. a)"
   ]
  },
  {
   "cell_type": "markdown",
   "metadata": {},
   "source": [
    "### 1. Leap frog in time, centred in space\n",
    "\n",
    "Considering the given one dimensional advection equation and applying the leap frog in time, centred in space scheme, we have:\n",
    "\n",
    "$$\\frac{u^{n+1}_{j} - u^{n-1}_{j}}{2\\Delta t} + c \\frac{u^{n}_{j+1} - u^{n}_{j-1}}{2\\Delta x} = 0 $$\n",
    "\n",
    "Using the hint $u^n_j = A\\lambda^n{\\rm e}^{ikj\\Delta x}$ yields to:\n",
    "\n",
    "$$\\frac{A e^{ikj\\Delta x} \\left(\\lambda^{n+1}-\\lambda^{n-1}\\right)}{2\\Delta t} + c\\frac{A\\lambda^{n}\\left(e^{ik\\Delta x(j+1)}-e^{ik\\Delta x(j-1)}\\right)}{2\\Delta x} = 0$$\n",
    "\n",
    "Dividing by $A$, $e^{ikj\\Delta x}$ and $\\lambda$ then leaves:\n",
    "\n",
    "$$\\lambda - \\lambda^{-1} + \\frac{c \\Delta t}{\\Delta x} \\left(e^{ik\\Delta x}-e^{-ik\\Delta x}\\right) = 0$$\n",
    "\n",
    "Using $e^{ikj\\Delta x} = \\cos(k\\Delta x) + i\\sin(k\\Delta x)$:\n",
    "\n",
    "$$\\lambda - \\lambda^{-1} + \\frac{c \\Delta t}{\\Delta x} \\left[\\cos(k\\Delta x)+i\\sin(k\\Delta x) - \\cos(k \\Delta x) + i\\sin(k \\Delta x)\\right] = 0$$\n",
    "\n",
    "Multiplying by $\\lambda$ and using $q = \\frac{c \\Delta t}{\\Delta x}$ yields:\n",
    "\n",
    "$$\\lambda^{2} + \\lambda 2qi\\sin(k\\Delta x) - 1 = 0$$\n",
    "\n",
    "Which we can solve using Bhaskara:\n",
    "\n",
    "\\begin{align}\n",
    "\\lambda &= \\frac{-b \\pm \\sqrt{b^{2}- 4ac}}{2a} \\notag \\\\\n",
    "&= \\frac{-2qi\\sin(k\\Delta x) \\pm \\sqrt{-4q^{2}\\sin^{2}(k\\Delta x) +4}}{2} \\notag \\\\\n",
    "&= -qi\\sin(k\\Delta x) \\pm \\sqrt{1-q^{2}\\sin^{2}(k\\Delta x)}\n",
    "\\end{align}\n",
    "\n",
    "We then have two roots for $\\lambda$:\n",
    "\n",
    "$$\\lambda_{1}= -qi\\sin(k\\Delta x) + \\sqrt{1-q^{2}\\sin^{2}(k\\Delta x)}$$\n",
    "\n",
    "$$ \\lambda_{2}=-qi\\sin(k\\Delta x) - \\sqrt{1-q^{2}\\sin^{2}(k\\Delta x)}$$\n",
    "\n",
    "or with $\\sigma = q \\sin (k \\Delta x)$:\n",
    "\n",
    "$$\\lambda_{1}= -i\\sigma + \\sqrt{1-\\sigma^{2}}$$\n",
    "\n",
    "$$\\lambda_{2}= -i\\sigma - \\sqrt{1-\\sigma^{2}}$$\n",
    "\n",
    "We have a stable solution if $\\mid\\lambda\\mid \\le 1$. We calculate the module of $\\lambda$ with $\\mid\\lambda\\mid = \\sqrt{Re(\\lambda)^{2} + Im(\\lambda)^{2}}$\n",
    "\n",
    "We have two possible cases: (1) $|\\sigma| \\le 1$ and  (2) $|\\sigma| > 1$\n",
    "\n",
    "For the first case, the root is solely real and thus:\n",
    "\n",
    "$$|\\lambda_{1}|=|\\lambda_{2}| = \\sqrt{\\sigma^{2}+\\sqrt{1-\\sigma^{2}}^{2}} = \\sqrt{\\sigma^{2}+1-\\sigma^{2}}=1$$\n",
    "\n",
    "The solution is unconditional stable within $|\\sigma| \\le 1$.\n",
    "\n",
    "For the second case, the root is solely imaginary and thus:\n",
    "\n",
    "$$\\lambda_{1,2} = i (-\\sigma \\pm \\sqrt{\\sigma^{2}-1})$$\n",
    "\n",
    "$$|\\lambda_{1,2}| = |(-\\sigma \\pm \\sqrt{\\sigma^{2}-1})|$$\n",
    "\n",
    "Together with the case condition $|\\sigma| > 1$ it is clear that depending on the sign of $\\sigma$, either $|\\lambda_{1}|>1$ or $|\\lambda_{2}|>1$. This means the solution is always unstable for this case. This leaves us with the final stablility criterion on $\\sigma$:\n",
    "\n",
    "$$|\\sigma| \\le 1$$\n",
    "\n",
    "To satisfy this for all possible values of $k$ we find:\n",
    "\n",
    "$$ -1 \\le \\frac{c\\Delta t}{\\Delta x} \\le 1$$"
   ]
  },
  {
   "cell_type": "markdown",
   "metadata": {},
   "source": [
    "### 2. Forward in time, upstream:\n",
    "\n",
    "Considering the given one dimensional advection equation and applying the forward in time, upstream scheme, we have:\n",
    "\n",
    "$$\\frac{u^{n+1}_{j} - u^{n}_{j}}{\\Delta t} + c \\frac{u^{n}_{j} - u^{n}_{j-1}}{\\Delta x} = 0 $$\n",
    "\n",
    "Using the hint $u^n_j = A\\lambda^n{\\rm e}^{ikj\\Delta x}$ yields to:\n",
    "\n",
    "$$\\frac{A e^{ikj\\Delta x} \\left(\\lambda^{n+1}-\\lambda^{n}\\right)}{\\Delta t} + c\\frac{A\\lambda^{n}\\left(e^{ik\\Delta xj}-e^{ik\\Delta x(j-1)}\\right)}{\\Delta x} = 0$$\n",
    "\n",
    "Dividing by $A$, $e^{ikj\\Delta x}$ and $\\lambda$ then leaves:\n",
    "\n",
    "$$\\lambda - 1 + \\frac{c\\Delta t}{\\Delta x} \\left(1-e^{-ik\\Delta x}\\right) = 0$$\n",
    "\n",
    "Using $e^{ikj\\Delta x} = \\cos(k\\Delta x) + i\\sin(k\\Delta x)$:\n",
    "\n",
    "\\begin{align}\n",
    "\\lambda &= 1 - \\frac{c\\Delta t}{\\Delta x} \\left[1 - \\cos(k\\Delta x) + \\sin(k\\Delta x)\\right] \\notag \\\\\n",
    "&= 1 + \\frac{c\\Delta t}{\\Delta x}\\left[\\cos(k\\Delta x) -1 \\right] -\\frac{c\\Delta t}{\\Delta x} i \\sin(k\\Delta x) \\notag \\\\\n",
    "\\end{align}\n",
    "\n",
    "Calculating the module of $\\lambda$, using $q = \\frac{c \\Delta t}{\\Delta x}$:\n",
    "\n",
    "\\begin{align}\n",
    "\\mid\\lambda\\mid &= \\sqrt{\\left\\{1 + q\\left[\\cos(k\\Delta x) -1 \\right]\\right\\}^{2} +\\left[-q \\sin(k\\Delta x)\\right]^{2}} \\notag \\\\\n",
    "&= \\sqrt{1 + 2q\\cos(k\\Delta x) -2q + q^{2}\\cos^{2}(k\\Delta x) - 2q^{2}\\cos(k\\Delta x) + q^{2} + q^{2}\\sin^{2}(k\\Delta x)} \\notag \\\\\n",
    "&= \\sqrt{1 + 2q^{2}[1 - \\cos(k\\Delta x)] + 2q[\\cos(k\\Delta x) -1]}\n",
    "\\end{align}\n",
    "\n",
    "For $\\mid\\lambda\\mid \\le 1$:\n",
    "\n",
    "$$1 + 2q^{2}[1 - \\cos(k\\Delta x)] + 2q[\\cos(k\\Delta x) -1] \\le 1$$\n",
    "\n",
    "$$q\\left\\{q\\left[1-\\cos(k\\Delta x)\\right]+\\cos(k\\Delta x)-1\\right\\} \\le 0$$\n",
    "\n",
    "Then for this scheme to be stable, the following condition must be satisfied:\n",
    "\n",
    "$$ 0 \\le \\frac{c\\Delta t}{\\Delta x} \\le 1$$"
   ]
  },
  {
   "cell_type": "markdown",
   "metadata": {},
   "source": [
    "### 3. Forward in time, downstream\n",
    "\n",
    "Considering the given one dimensional advection equation and applying the forward in time, upstream scheme, we have:\n",
    "\n",
    "$$\\frac{u^{n+1}_{j} - u^{n}_{j}}{\\Delta t} + c \\frac{u^{n}_{j+1} - u^{n}_{j}}{\\Delta x} = 0 $$\n",
    "\n",
    "Using the hint $u^n_j = A\\lambda^n{\\rm e}^{ikj\\Delta x}$ yields to:\n",
    "\n",
    "$$\\frac{A e^{ikj\\Delta x} \\left(\\lambda^{n+1}-\\lambda^{n}\\right)}{\\Delta t} + c\\frac{A\\lambda^{n}\\left(e^{ik\\Delta x(j+1)}-e^{ik\\Delta xj}\\right)}{\\Delta x} = 0$$\n",
    "\n",
    "Dividing by $A$, $e^{ikj\\Delta x}$ and $\\lambda$ then leaves:\n",
    "\n",
    "$$(\\lambda-1) + \\frac{c\\Delta t}{\\Delta x} \\left(e^{ik\\Delta x}-1\\right) = 0$$\n",
    "\n",
    "Using $e^{ikj\\Delta x} = \\cos(k\\Delta x) + i\\sin(k\\Delta x)$:\n",
    "\n",
    "\\begin{align}\n",
    "\\lambda &= 1 - \\frac{c\\Delta t}{\\Delta x} \\left[\\cos(k\\Delta x) + \\sin(k\\Delta x) -1\\right] \\notag \\\\\n",
    "&= 1 - \\frac{c\\Delta t}{\\Delta x}\\left[\\cos(k\\Delta x) -1 \\right] -\\frac{c\\Delta t}{\\Delta x} i \\sin(k\\Delta x) \\notag \\\\\n",
    "\\end{align}\n",
    "\n",
    "Calculating the module of $\\lambda$, using $q = \\frac{c \\Delta t}{\\Delta x}$:\n",
    "\n",
    "\\begin{align}\n",
    "\\mid\\lambda\\mid &= \\sqrt{\\left\\{1-q\\left[\\cos(k\\Delta x) -1\\right]\\right\\}^{2} +\\left[q\\sin(k\\Delta x)\\right]^{2}} \\notag \\\\\n",
    "&= \\sqrt{1-2q\\left[\\cos(k\\Delta x)-1\\right] +q^{2}\\cos^{2}(k\\Delta x) -2q^{2}\\cos(k\\Delta x) +q^{2} + q^{2}\\sin^{2}(k\\Delta x)} \\notag \\\\\n",
    "&= \\sqrt{1+q^{2}\\left[2-2\\cos(k\\Delta x)\\right] - 2q\\left[\\cos(k\\Delta x) -1\\right]}\n",
    "\\end{align}\n",
    "\n",
    "For $\\mid\\lambda\\mid \\le 1$:\n",
    "\n",
    "$$1+q^{2}\\left[2-2\\cos(k\\Delta x)\\right] - 2q\\left[\\cos(k\\Delta x) -1\\right] \\le 1$$\n",
    "\n",
    "$$q^{2}\\left[2-2\\cos(k\\Delta x)\\right] - 2q\\left[\\cos(k\\Delta x) -1\\right] \\le 0$$\n",
    "\n",
    "$$q\\left\\{q\\left[1-cos(k\\Delta x)\\right] - \\left[\\cos(k\\Delta x) - 1\\right]\\right\\} \\le 0 $$\n",
    "\n",
    "Then for this scheme to be stable, the following condition must be satisfied:\n",
    "\n",
    "$$ -1 \\le \\frac{c\\Delta t}{\\Delta x} \\le 0$$"
   ]
  },
  {
   "cell_type": "code",
   "execution_count": null,
   "metadata": {},
   "outputs": [],
   "source": []
  }
 ],
 "metadata": {
  "kernelspec": {
   "display_name": "Python [conda env:ws20climnum]",
   "language": "python",
   "name": "conda-env-ws20climnum-py"
  },
  "language_info": {
   "codemirror_mode": {
    "name": "ipython",
    "version": 3
   },
   "file_extension": ".py",
   "mimetype": "text/x-python",
   "name": "python",
   "nbconvert_exporter": "python",
   "pygments_lexer": "ipython3",
   "version": "3.7.8"
  }
 },
 "nbformat": 4,
 "nbformat_minor": 4
}
